Is0/Lemmas.lean
@@ -9,19 +9,19 @@ import Is0.Programs
 
 namespace Risc0
 
-section WithCirgen 
+section WithMLIR 
 
-open CirgenNotation
+open MLIRNotation
 
-lemma Cirgen.run_Sequence_Assign_collapsible {state : State} {name : String} {op : Op} {program : Cirgen} :
+lemma MLIR.run_Sequence_Assign_collapsible {state : State} {name : String} {op : Op} {program : MLIR} :
     Γ state ⟦name ←ₐ op; program⟧ = Γ (state[name] := Γ state ⟦op⟧) ⟦program⟧ := by
-  cases op <;> conv => lhs; simp [Cirgen.run, State.update, Map.update, beq_iff_eq]
+  cases op <;> conv => lhs; simp [MLIR.run, State.update, Map.update, beq_iff_eq]
 
-lemma Cirgen.run_Sequence_Set_collapsible
+lemma MLIR.run_Sequence_Set_collapsible
     {state : State}
     {name : String}
     {nameₓ : String}
-    {program : Cirgen}
+    {program : MLIR}
     (buffer : List Felt)
     (x : Felt)
     (h : state.buffers name = some buffer)
@@ -29,7 +29,7 @@ lemma Cirgen.run_Sequence_Set_collapsible
     Γ state ⟦⟨name⟩[i] ←ₐ ⟨nameₓ⟩; program⟧ = 
     Γ { state with buffers := state.buffers[name] := buffer.set i x } ⟦program⟧ := by simp [run, *]
 
-lemma Cirgen.run_if_true {c : Variable Felt}
+lemma MLIR.run_if_true {c : Variable Felt}
   (h : st.felts c.name = some 0) :
   Γ st ⟦guard c then prog⟧ = (st, none) := by
   simp only [run]; generalize eq : st.felts c.name = cond
@@ -37,7 +37,7 @@ lemma Cirgen.run_if_true {c : Variable Felt}
   · cases h
   · simp; exact λ contra => absurd (by injection h) contra
 
-lemma Cirgen.run_if_false {c : Variable Felt}
+lemma MLIR.run_if_false {c : Variable Felt}
   (x : Felt)
   (h₁ : st.felts c.name = some x)
   (h₂ : x ≠ 0) :
@@ -50,17 +50,17 @@ lemma Cirgen.run_if_false {c : Variable Felt}
     injection h₁ with contra
     exact absurd contra.symm h₂
 
-lemma Cirgen.run_seq :
+lemma MLIR.run_seq :
   Γ st ⟦p₁; p₂⟧ = let (st', x) := Γ st ⟦p₁⟧
                   match x with
                     | some x => (st', some x)
                     | none => Γ st' ⟦p₂⟧ := rfl
 
-lemma Cirgen.run_Sequence_If_collapsible
+lemma MLIR.run_Sequence_If_collapsible
     {state : State}
     {name : String}
-    {branch : Cirgen}
-    {program : Cirgen}
+    {branch : MLIR}
+    {program : MLIR}
     (x : Felt)
     (h₁ : state.felts name = some x)
     : Γ state ⟦guard ⟨name⟩ then branch; program⟧
@@ -73,18 +73,18 @@ lemma Cirgen.run_Sequence_If_collapsible
     · rw [run_if_false x h₁ (by simp at eq; exact eq)]; rfl
     · rw [run_if_true (by simp at eq; rw [eq] at h₁; exact h₁)]; rfl
 
-lemma Cirgen.run_If_collapsible
+lemma MLIR.run_If_collapsible
     {state : State}
     {name : String}
-    {branch : Cirgen}
+    {branch : MLIR}
     (x : Felt)
     (h₁ : state.felts name = some x) :
     Γ state ⟦guard ⟨name⟩ then branch⟧
   = if (x == 0)
       then (state, none)
-      else Cirgen.run state branch := by simp [run, h₁]
+      else MLIR.run state branch := by simp [run, h₁]
 
-lemma Cirgen.run_Eqz_collapsible
+lemma MLIR.run_Eqz_collapsible
     {state : State}
     {name : String}
     (x : Felt)
@@ -92,17 +92,17 @@ lemma Cirgen.run_Eqz_collapsible
     Γ state ⟦?₀ ⟨name⟩⟧ 
   = ({ state with constraints := x :: state.constraints }, none) := by simp [run, *]
 
-lemma Cirgen.run_Sequence_Eqz_collapsible
+lemma MLIR.run_Sequence_Eqz_collapsible
     {state : State}
     {name : String}
-    {program : Cirgen}
+    {program : MLIR}
     (x : Felt)
     (h₁ : state.felts name = some x) :
-    Cirgen.run state (.Sequence (.Eqz (Variable.mk name)) program)
+    MLIR.run state (.Sequence (.Eqz (Variable.mk name)) program)
   = let state₁ := { state with constraints := x :: state.constraints }
-    let (state₂, y) := Cirgen.run state₁ program
+    let (state₂, y) := MLIR.run state₁ program
     (state₂, y) := by rw [run_seq, run_Eqz_collapsible _ h₁]
 
-end WithCirgen 
+end WithMLIR 
 
 end Risc0
